A number of renaming changes in UF: UF's GeneralGraph was being called "Graph", which is a bit too general and is also something like a keyword. Changed to "UFGraph" instead. Made progress in Kruskal's VST proof.

msl_application/UnionFindGraph.v
@@ -33,17 +33,17 @@ Section UnionFindGraph.
   Context {DV DE DG: Type}.
 
   Definition LGraph := LabeledGraph V E DV DE DG.
-  Definition Graph := (GeneralGraph V E DV DE DG (fun g => LiMaFin (pg_lg g))).
+  Definition UFGraph := (GeneralGraph V E DV DE DG (fun g => LiMaFin (pg_lg g))).
 
-  Definition Graph_LGraph (G: Graph): LGraph := lg_gg G.
+  Definition UFGraph_LGraph (G: UFGraph): LGraph := lg_gg G.
 
-  Local Coercion Graph_LGraph: Graph >-> LGraph.
+  Local Coercion UFGraph_LGraph: UFGraph >-> LGraph.
   Local Identity Coercion LGraph_LabeledGraph: LGraph >-> LabeledGraph.
   Local Coercion pg_lg: LabeledGraph >-> PreGraph.
 
-  Instance maGraph(G: Graph): MathGraph G isNullDec := @ma G (@sound_gg _ _ _ _ _ _ _ _ G).
-  Instance finGraph (G: Graph): FiniteGraph G := @fin G (@sound_gg _ _ _ _ _ _ _ _ G).
-  Instance liGraph (G: Graph):  LstGraph G out_edge := @li G (@sound_gg _ _ _ _ _ _ _ _ G).
+  Instance maGraph(G: UFGraph): MathGraph G isNullDec := @ma G (@sound_gg _ _ _ _ _ _ _ _ G).
+  Instance finGraph (G: UFGraph): FiniteGraph G := @fin G (@sound_gg _ _ _ _ _ _ _ _ G).
+  Instance liGraph (G: UFGraph):  LstGraph G out_edge := @li G (@sound_gg _ _ _ _ _ _ _ _ G).
 
   (*Returns the rank (vlabel) and parent of a vertex
     Parent is: take (any?) dst x has an edge to.
@@ -53,7 +53,7 @@ Section UnionFindGraph.
   Definition vgamma (g: LGraph) (x: V) : DV * V := (vlabel g x, let target := dst (pg_lg g) (out_edge x) in if (projT2 isNullDec target) then x else target).
 
   (*If v is in graph, and vgamma g v = some rank and parent, then the parent is also valid. *)
-  Lemma valid_parent: forall (g: Graph) v n p, vvalid g v -> vgamma g v = (n, p) -> vvalid g p.
+  Lemma valid_parent: forall (g: UFGraph) v n p, vvalid g v -> vgamma g v = (n, p) -> vvalid g p.
   Proof.
     intros. unfold vgamma in H0. simpl in H0. inversion H0. clear H0 H2. destruct (projT2 isNullDec (dst g (out_edge v))); auto.
     assert (~ isNullDec (dst g (out_edge v))) by (intro; apply n0; auto).
@@ -61,14 +61,14 @@ Section UnionFindGraph.
     pose proof (valid_graph _ _ H4). destruct H5 as [_ [? | ?]]; auto. exfalso; auto.
   Qed.
 
-  Lemma parent_loop: forall (g: Graph) v n y, vgamma g v = (n, v) -> reachable g v y -> v = y.
+  Lemma parent_loop: forall (g: UFGraph) v n y, vgamma g v = (n, v) -> reachable g v y -> v = y.
   Proof.
     intros. unfold vgamma in H. destruct (projT2 isNullDec (dst g (out_edge v))).
     - apply (lst_out_edge_only_one g _ v (dst g (out_edge v)) y); auto. intro. apply reachable_head_valid in H1. apply (valid_not_null g (dst g (out_edge v)) H1); auto.
     - apply (lst_self_loop _ (liGraph g)) in H0; auto. inversion H. rewrite H3. auto.
   Qed.
 
-  Lemma gamma_parent_reachable_included: forall (g: Graph) x r pa, vvalid g x -> vgamma g x = (r, pa) -> Included (reachable g pa) (reachable g x).
+  Lemma gamma_parent_reachable_included: forall (g: UFGraph) x r pa, vvalid g x -> vgamma g x = (r, pa) -> Included (reachable g pa) (reachable g x).
   Proof.
     intros. intro y; intros. unfold vgamma in H0. destruct (projT2 isNullDec (dst g (out_edge x))).
     - inversion H0. auto.
@@ -77,7 +77,7 @@ Section UnionFindGraph.
       + inversion H0. rewrite H4. rewrite (dst_step _ (liGraph g) _ _ H H4). auto.
   Qed.
 
-  Lemma Prop_join_reachable_parent: forall (g: Graph) x r pa,
+  Lemma Prop_join_reachable_parent: forall (g: UFGraph) x r pa,
       vvalid g x -> vgamma g x = (r, pa) ->
       Prop_join
         (reachable g pa)
@@ -93,7 +93,7 @@ Section UnionFindGraph.
       + apply FiniteGraph_EnumCovered; auto.
   Qed.
 
-  Definition Graph_gen_redirect_parent (g: Graph) (x: V) (pa: V) (H: weak_valid g pa) (Hv: vvalid g x) (Hn: ~ reachable g pa x): Graph.
+  Definition Graph_gen_redirect_parent (g: UFGraph) (x: V) (pa: V) (H: weak_valid g pa) (Hv: vvalid g x) (Hn: ~ reachable g pa x): UFGraph.
   Proof.
     refine (generalgraph_gen_dst g (out_edge x) pa _). constructor.
     - simpl. apply (gen_dst_preserve_lst g (liGraph g)); auto.
@@ -101,7 +101,7 @@ Section UnionFindGraph.
     - apply (gen_dst_preserve_finite g (out_edge x) pa (finGraph g)).
   Defined.
 
-  Lemma Graph_reachable_dec: forall (G: Graph) x, Decidable (vvalid G x) -> forall y, Decidable (reachable G x y).
+  Lemma Graph_reachable_dec: forall (G: UFGraph) x, Decidable (vvalid G x) -> forall y, Decidable (reachable G x y).
   Proof.
     intros. apply reachable_decidable with (is_null := isNullDec); auto.
     + apply maGraph.
@@ -109,28 +109,28 @@ Section UnionFindGraph.
     + apply FiniteGraph_EnumCovered, finGraph.
   Qed.
 
-  Definition Graph_vgen (G: Graph) (x: V) (d: DV) : Graph := generalgraph_vgen G x d (sound_gg G).
+  Definition Graph_vgen (G: UFGraph) (x: V) (d: DV) : UFGraph := generalgraph_vgen G x d (sound_gg G).
 
-  Lemma uf_root_vgamma: forall (g: Graph) v n, vvalid g v -> vgamma g v = (n, v) -> uf_root g v v.
+  Lemma uf_root_vgamma: forall (g: UFGraph) v n, vvalid g v -> vgamma g v = (n, v) -> uf_root g v v.
   Proof. intros. split; [apply reachable_refl | intros; apply (parent_loop g _ n)]; auto. Qed.
 
-  Lemma vgamma_not_dst: forall (g: Graph) x r pa, vgamma g x = (r, pa) -> pa <> x -> dst g (out_edge x) = pa.
+  Lemma vgamma_not_dst: forall (g: UFGraph) x r pa, vgamma g x = (r, pa) -> pa <> x -> dst g (out_edge x) = pa.
   Proof. intros. unfold vgamma in H. destruct (projT2 isNullDec (dst g (out_edge x))); inversion H; [exfalso |]; auto. Qed.
 
-  Lemma vgamma_not_edge: forall (g: Graph) x r pa, vvalid g x -> vgamma g x = (r, pa) -> pa <> x -> g |= x ~> pa.
+  Lemma vgamma_not_edge: forall (g: UFGraph) x r pa, vvalid g x -> vgamma g x = (r, pa) -> pa <> x -> g |= x ~> pa.
   Proof.
     intros. assert (vvalid g pa) by (apply valid_parent in H0; auto). hnf. split; [|split]; auto.
     apply (vgamma_not_dst g x r) in H1; auto. rewrite step_spec. exists (out_edge x).
     pose proof (vvalid_src_evalid _ (liGraph g) _ H). destruct H3. split; auto.
   Qed.
 
-  Lemma vgamma_not_reachable': forall (g: Graph) x r pa y, vvalid g x -> vgamma g x = (r, pa) -> pa <> x -> reachable g pa y -> ~ reachable g y x.
+  Lemma vgamma_not_reachable': forall (g: UFGraph) x r pa y, vvalid g x -> vgamma g x = (r, pa) -> pa <> x -> reachable g pa y -> ~ reachable g y x.
   Proof. intros. apply (dst_not_reachable _ (liGraph g) _ pa); auto. apply (vgamma_not_dst g x r); auto. Qed.
 
-  Lemma vgamma_not_reachable: forall (g: Graph) x r pa, vvalid g x -> vgamma g x = (r, pa) -> pa <> x -> ~ reachable g pa x.
+  Lemma vgamma_not_reachable: forall (g: UFGraph) x r pa, vvalid g x -> vgamma g x = (r, pa) -> pa <> x -> ~ reachable g pa x.
   Proof. intros. assert (vvalid g pa) by (apply valid_parent in H0; auto). apply (vgamma_not_reachable' g x r pa pa); auto. apply reachable_refl; auto. Qed.
   
-  Lemma uf_root_not_eq_root_vgamma: forall (g: Graph) x r pa root, vgamma g x = (r, pa) -> uf_root g x root -> x <> root -> x <> pa.
+  Lemma uf_root_not_eq_root_vgamma: forall (g: UFGraph) x r pa root, vgamma g x = (r, pa) -> uf_root g x root -> x <> root -> x <> pa.
   Proof.
     intros. unfold vgamma in H. destruct (projT2 isNullDec (dst g (out_edge x))). 
     - destruct H0. apply reachable_ind.reachable_ind in H0. destruct H0. 1: exfalso; auto. destruct H0 as [z [[? [? ?]] [? ?]]]. rewrite step_spec in H4.
@@ -144,7 +144,7 @@ Section UnionFindGraph.
       } rewrite H4. intro. rewrite <- H3 in H2. apply (@no_loop_path _ _ _ _ g _ (liGraph g)) in H2. inversion H2.
   Qed.
 
-  Lemma vgamma_uf_root: forall (g: Graph) x r pa root, vvalid g x -> vgamma g x = (r, pa) -> uf_root g x root -> x <> root -> uf_root g pa root.
+  Lemma vgamma_uf_root: forall (g: UFGraph) x r pa root, vvalid g x -> vgamma g x = (r, pa) -> uf_root g x root -> x <> root -> uf_root g pa root.
   Proof.
     intros. pose proof (uf_root_not_eq_root_vgamma g _ _ _ _ H0 H1 H2). destruct H1. split; auto. pose proof (valid_parent g _ _ _ H H0).  
     assert (Decidable (reachable g pa root)) by (apply Graph_reachable_dec; left; auto). apply decidable_prop_decidable in H6. destruct H6; auto. exfalso.
@@ -155,32 +155,32 @@ Section UnionFindGraph.
 
   Global Existing Instance fml.
 
-  Lemma findS_preserves_vgamma: forall (g1 g2: Graph) x r pa, vvalid g1 x -> vgamma g1 x = (r, pa) -> pa <> x -> findS g1 pa g2 -> vgamma g2 x = (r, pa).
+  Lemma findS_preserves_vgamma: forall (g1 g2: UFGraph) x r pa, vvalid g1 x -> vgamma g1 x = (r, pa) -> pa <> x -> findS g1 pa g2 -> vgamma g2 x = (r, pa).
   Proof.
     intros. assert (Hr: ~ reachable g1 pa x) by (apply vgamma_not_reachable with r; auto). unfold vgamma in *. destruct (projT2 isNullDec (dst g1 (out_edge x))).
     1: inversion H0; exfalso; auto. rewrite <- H0. destruct H2 as [? [[? ?] ?]]. f_equal.
-    - assert (vvalid g2 x) by (rewrite <- H3; auto). specialize (H5 x H H6). unfold Graph_LGraph. rewrite H5. auto.
+    - assert (vvalid g2 x) by (rewrite <- H3; auto). specialize (H5 x H H6). unfold UFGraph_LGraph. rewrite H5. auto.
     - assert (evalid (predicate_partialgraph (lg_gg g1) (fun n : V => ~ reachable (lg_gg g1) pa n)) (out_edge x)). {
-        simpl. hnf. pose proof (vvalid_src_evalid _ (liGraph g1) _ H). unfold Graph_LGraph in H6. destruct H6. rewrite H6. split; auto.
-      } destruct H2 as [_ [? [_ ?]]]. pose proof H6. rewrite H2 in H8. clear H2. specialize (H7 _ H6 H8). simpl in H7. unfold Graph_LGraph. rewrite <- H7.
+        simpl. hnf. pose proof (vvalid_src_evalid _ (liGraph g1) _ H). unfold UFGraph_LGraph in H6. destruct H6. rewrite H6. split; auto.
+      } destruct H2 as [_ [? [_ ?]]]. pose proof H6. rewrite H2 in H8. clear H2. specialize (H7 _ H6 H8). simpl in H7. unfold UFGraph_LGraph. rewrite <- H7.
       destruct (projT2 isNullDec (dst (lg_gg g1) (out_edge x))); [exfalso |]; auto.
   Qed.
 
-  Lemma the_same_root_union: forall (g g1 g2: Graph) x y root,
+  Lemma the_same_root_union: forall (g g1 g2: UFGraph) x y root,
       vvalid g x -> vvalid g y -> uf_equiv g g1 -> uf_equiv g1 g2 -> uf_root g1 x root -> uf_root g2 y root -> uf_union g x y g2.
   Proof. intros. apply (same_root_union g g1 g2 x y root); auto. Qed.
 
-  Lemma uf_equiv_root_the_same: forall (g1 g2: Graph) x root, uf_equiv g1 g2 -> uf_root g1 x root <-> uf_root g2 x root.
+  Lemma uf_equiv_root_the_same: forall (g1 g2: UFGraph) x root, uf_equiv g1 g2 -> uf_root g1 x root <-> uf_root g2 x root.
   Proof. intros. pose proof (@uf_equiv_the_same_root _ _ _ _ _ _ _ _ out_edge isNullDec fml g1 g2 x root H). apply H0. Qed.
 
-  Lemma uf_equiv_not_reachable: forall (g1 g2: Graph) x r pa root,
+  Lemma uf_equiv_not_reachable: forall (g1 g2: UFGraph) x r pa root,
       vvalid g1 x -> vgamma g1 x = (r, pa) -> pa <> x -> uf_equiv g1 g2 -> uf_root g2 pa root -> ~ reachable g2 root x.
   Proof.
     intros. pose proof H3. rewrite <- (uf_equiv_root_the_same _ _ pa root H2) in H4. destruct H3. intro. apply H5 in H6. subst x.
     pose proof (vgamma_not_reachable g1 root r pa H H0 H1). destruct H4. auto.
   Qed.
 
-  Lemma graph_gen_redirect_parent_equiv': forall (g1 g2: Graph) x root,
+  Lemma graph_gen_redirect_parent_equiv': forall (g1 g2: UFGraph) x root,
       uf_equiv g1 g2 -> vvalid g2 x -> (~ reachable g2 root x) -> uf_root g2 x root -> uf_equiv g1 (pregraph_gen_dst g2 (out_edge x) root).
   Proof.
     intros. apply (@uf_equiv_trans _ _ _ _ g2 _ (liGraph g2) _ (maGraph g2) (finGraph g2)); auto. split; intro y; simpl; [intuition |]. intros.
@@ -192,14 +192,14 @@ Section UnionFindGraph.
     - apply (uf_root_unique _ (gen_dst_preserve_lst g2 (liGraph g2) _ _ H1 H0) y); auto. apply (uf_root_gen_dst_preserve g2 (liGraph g2)); auto.
   Qed.
 
-  Lemma graph_gen_redirect_parent_equiv: forall (g1 g2: Graph) x r pa root (Hv: vvalid g2 x) (Hn: ~ reachable g2 root x),
+  Lemma graph_gen_redirect_parent_equiv: forall (g1 g2: UFGraph) x r pa root (Hv: vvalid g2 x) (Hn: ~ reachable g2 root x),
       vvalid g1 x -> vgamma g1 x = (r, pa) -> pa <> x -> uf_equiv g1 g2 -> uf_root g2 pa root -> uf_equiv g1 (pregraph_gen_dst g2 (out_edge x) root).
   Proof.
     intros. apply graph_gen_redirect_parent_equiv'; auto. rewrite <- (uf_equiv_root_the_same g1); auto.
     apply (uf_root_edge g1 (liGraph g1) x pa); [| apply (vgamma_not_dst g1 x r) | rewrite (uf_equiv_root_the_same g1 g2)]; auto.
   Qed.
 
-  Lemma graph_gen_redirect_parent_findS: forall (g1 g2: Graph) x r1 r2 pa pa' (H: weak_valid g2 pa') (Hv: vvalid g2 x) (Hn: ~ reachable g2 pa' x),
+  Lemma graph_gen_redirect_parent_findS: forall (g1 g2: UFGraph) x r1 r2 pa pa' (H: weak_valid g2 pa') (Hv: vvalid g2 x) (Hn: ~ reachable g2 pa' x),
       vvalid g1 x -> vgamma g1 x = (r1, pa) -> pa <> x -> vgamma g2 x = (r2, pa) -> findS g1 pa g2 -> uf_root g2 pa pa' ->
       findS g1 x (Graph_gen_redirect_parent g2 x pa' H Hv Hn).
   Proof.
@@ -218,20 +218,20 @@ Section UnionFindGraph.
       + split; intros; destruct H13.
         * pose proof (H8 _ H14). pose proof (conj H13 H15). rewrite H10 in H16. destruct H16. rewrite H9 in H17. destruct H17. 1: split; auto. symmetry in H17.
           pose proof (conj H17 H16). rewrite (@only_one_edge _ _ _ _ g2 _ (liGraph g2)) in H18; auto. subst e. pose proof (vvalid_src_evalid _ (liGraph g1) _ H0).
-          destruct H18 as [? _]. unfold Graph_LGraph in H18. rewrite H18 in H14. exfalso. apply H14. apply reachable_refl. auto.
+          destruct H18 as [? _]. unfold UFGraph_LGraph in H18. rewrite H18 in H14. exfalso. apply H14. apply reachable_refl. auto.
         * pose proof (H8 _ H14). pose proof (conj H13 H15). rewrite <- H10 in H16. destruct H16. rewrite H9 in H17. destruct H17. 1: split; auto. symmetry in H17.
           pose proof (conj H17 H16). rewrite (@only_one_edge _ _ _ _ g1 _ (liGraph g1)) in H18; auto. subst e. pose proof (vvalid_src_evalid _ (liGraph g2) _ Hv).
-          destruct H18 as [? _]. unfold Graph_LGraph in H18. rewrite H18 in H14. exfalso. apply H14. apply reachable_refl. auto.
+          destruct H18 as [? _]. unfold UFGraph_LGraph in H18. rewrite H18 in H14. exfalso. apply H14. apply reachable_refl. auto.
       + destruct H13, H14. apply H8 in H15. apply H8 in H16. apply H11; auto.
       + unfold updateEdgeFunc. destruct (equiv_dec (out_edge x) e).
         * unfold Equivalence.equiv in e0. subst e. pose proof (vvalid_src_evalid _ (liGraph g1) _ H0).
-          destruct H15. unfold Graph_LGraph in H15. destruct H13. exfalso. apply H17. rewrite H15. apply reachable_refl; auto.
+          destruct H15. unfold UFGraph_LGraph in H15. destruct H13. exfalso. apply H17. rewrite H15. apply reachable_refl; auto.
         * destruct H13, H14. apply H8 in H15. apply H8 in H16. apply H12; auto.
     - apply (graph_gen_redirect_parent_equiv _ _ _ r1 pa); auto.
     - apply H7.
   Qed.
 
-  Lemma diff_root_union_1: forall (g g1 g2: Graph) x y x_root y_root,
+  Lemma diff_root_union_1: forall (g g1 g2: UFGraph) x y x_root y_root,
       uf_equiv g g1 -> uf_root g1 x x_root -> uf_equiv g1 g2 -> uf_root g2 y y_root -> x_root <> y_root ->
       (@weak_valid _ _ _ _ g2 _ (maGraph g2) y_root) -> vvalid g2 x_root ->
       ~ reachable g2 y_root x_root -> uf_union g x y (pregraph_gen_dst g2 (out_edge x_root) y_root).
@@ -241,7 +241,7 @@ Section UnionFindGraph.
     apply (@diff_root_union _ _ _ _ _ _ _ _ out_edge isNullDec fml); auto. apply (uf_equiv_root_the_same g1); auto.
   Qed.
 
-  Lemma diff_root_union_2: forall (g g1 g2: Graph) x y x_root y_root,
+  Lemma diff_root_union_2: forall (g g1 g2: UFGraph) x y x_root y_root,
       uf_equiv g g1 -> uf_root g1 x x_root -> uf_equiv g1 g2 -> uf_root g2 y y_root -> x_root <> y_root -> (@weak_valid _ _ _ _ g2 _ (maGraph g2) x_root) -> vvalid g2 y_root ->
       ~ reachable g2 x_root y_root -> uf_union g x y (pregraph_gen_dst g2 (out_edge y_root) x_root).
   Proof.
@@ -250,7 +250,7 @@ Section UnionFindGraph.
     apply (@diff_root_union _ _ _ _ _ _ _ _ out_edge isNullDec fml); auto. apply (uf_equiv_root_the_same g1); auto.
   Qed.
 
-  Lemma graph_gen_redirect_parent_vgamma: forall (g1 g2: Graph) x r pa y (H: weak_valid g1 x) (Hv: vvalid g1 y) (Hn: ~ reachable g1 x y),
+  Lemma graph_gen_redirect_parent_vgamma: forall (g1 g2: UFGraph) x r pa y (H: weak_valid g1 x) (Hv: vvalid g1 y) (Hn: ~ reachable g1 x y),
       (forall a b, out_edge a = out_edge b -> a = b) -> vgamma g1 x = (r, pa) -> g2 = (Graph_gen_redirect_parent g1 y x H Hv Hn) -> vgamma g2 x = (r, pa).
   Proof.
     intros. rewrite H2. clear H2. unfold vgamma in *. simpl in *. inversion H1. f_equal. unfold updateEdgeFunc.
